Modified implementation of Types.subst

STLC/Constraint.v
@@ -1,19 +1,11 @@
-Require Import List Recdef Omega Finite_sets_facts.
+Require Import List Recdef Omega.
 Require Id Types.
 
 Lemma Forall_map : forall X Y (P : Y -> Prop) (f : X -> Y) l,
   Forall P (map f l) <-> Forall (fun x => P (f x)) l.
 Proof.
   intros ? ? ? ? l.
-  split; intros H.
-  - apply Forall_forall.
-    intros ? ?.
-    Hint Resolve in_map.
-    eapply Forall_forall in H; eauto.
-  - induction l;
-    simpl;
-    inversion H;
-    eauto.
+  split; intros H; induction l; simpl in *; inversion H; eauto.
 Qed.
 
 Definition t := list (Types.t * Types.t).
@@ -26,17 +18,15 @@ Notation size c :=
   (fold_right plus 0 (map (fun p =>
     Types.size (fst p) + Types.size (snd p)) c)).
 
-Notation subst x t c :=
-  (map (fun p => (Types.subst x t (fst p), Types.subst x t (snd p))) c).
-
-Notation subst_list s c :=
-  (map (fun p => (Types.subst_list s (fst p), Types.subst_list s (snd p))) c).
+Notation subst s c :=
+  (map (fun p => (Types.subst s (fst p), Types.subst s (snd p))) c).
 
 Notation unifies s c :=
-  (Forall (fun p => Types.unifies s (fst p) (snd p)) c).
+  (Forall (fun p => Types.subst s (fst p) = Types.subst s (snd p)) c).
 
-Lemma subst_occur : forall x t c,
-  Id.FSet.In x (FV (subst x t c)) -> Id.FSet.In x (Types.FV t).
+Lemma subst_FV : forall x s c,
+  Id.FSet.In x (FV (subst s c)) ->
+  exists y, Id.FSet.In x (Types.FV (s y)) /\ Id.FSet.In y (FV c).
 Proof.
   intros ? ? c H.
   induction c as [| [] ]; simpl in *.
@@ -44,40 +34,10 @@ Proof.
   - apply Id.FSet.union_spec in H.
     destruct H as [ H | H ].
     + apply Id.FSet.union_spec in H.
-      Hint Resolve Types.subst_occur.
-      destruct H; eauto.
-    + eauto.
+      destruct H as [H | H];
+      destruct (Types.subst_FV _ _ _ H) as [? []]; eauto 7.
+    + destruct (IHc H) as [? []]; eauto.
 Qed.
-
-Lemma subst_fv : forall x y t c,
-  Id.FSet.In x (FV (subst y t c)) -> Id.FSet.In x (Types.FV t) \/ Id.FSet.In x (FV c).
-Proof.
-  intros ? ? ? c H.
-  induction c as [| [] ]; simpl in *.
-  - destruct (Id.FSet.empty_spec H).
-  - apply Id.FSet.union_spec in H.
-    destruct H as [ H | H ].
-    + apply Id.FSet.union_spec in H.
-      destruct H as [ H | H ];
-      destruct (Types.subst_fv _ _ _ _ H); eauto 6.
-    + destruct (IHc H); eauto.
-Qed.
-
-Lemma subst_preserves_unifies : forall x t0 s c,
-  Types.unifies s (Types.Var x) t0 ->
-  unifies s c ->
-  unifies s (subst x t0 c).
-Proof.
-  intros ? ? ? ? ? ?.
-  apply Forall_map.
-  eapply Forall_impl; [| eauto ].
-  intros [] ?.
-  simpl in *.
-  repeat rewrite <- Types.subst_preserves_unifies;
-  eauto.
-Qed.
-
-Hint Resolve subst_preserves_unifies.
 
 Definition lt c1 c2 :=
   (Id.FSet.cardinal (FV c1) <= Id.FSet.cardinal (FV c2)) /\
@@ -86,18 +46,24 @@ Definition lt c1 c2 :=
 Lemma lt_subst : forall c x t t1 t2,
   ~Id.FSet.In x (Types.FV t) ->
   (t1 = t /\ t2 = Types.Var x \/ t1 = Types.Var x /\ t2 = t) ->
-  lt (subst x t c) ((t1, t2) :: c).
+  lt (subst (Types.subst_single x t) c) ((t1, t2) :: c).
 Proof.
   intros c x t ? ? Hmem Heq.
-  assert (Hcardinal : Id.FSet.cardinal (FV (subst x t c)) < Id.FSet.cardinal (FV ((t1, t2) :: c))).
+  assert (Hcardinal : Id.FSet.cardinal (FV (subst (Types.subst_single x t) c)) < Id.FSet.cardinal (FV ((t1, t2) :: c))).
   - apply Id.FSetProperties.subset_cardinal_lt with (x := x); simpl.
     + intros y HIn.
-      destruct (subst_fv _ _ _ _ HIn);
-      destruct Heq as [[] | []]; subst; eauto.
+      destruct (subst_FV _ _ _ HIn) as [z [H]].
+      unfold Types.subst_single in *.
+      destruct (Id.eq_dec x z);
+      [| apply Id.FSet.singleton_spec in H ];
+      destruct Heq as [[] | []]; subst; simpl in *; eauto.
     + destruct Heq as [[] | []]; subst; simpl; eauto 6.
     + intros Hoccur.
-      apply subst_occur in Hoccur.
-      eauto.
+      destruct (subst_FV _ _ _ Hoccur) as [z [H]].
+      unfold Types.subst_single in *.
+      destruct (Id.eq_dec x z);
+      [| apply Id.FSet.singleton_spec in H ];
+      subst; eauto.
   - split; omega.
 Qed.
 
@@ -154,48 +120,51 @@ Proof.
     omega.
 Qed.
 
-Function unify c { wf lt c } :=
+Function unify_aux c { wf lt c } :=
   match c with
   | nil => Some nil
   | (t1, t2) :: c' =>
-      if Types.eq_dec t1 t2 then unify c'
+      if Types.eq_dec t1 t2 then unify_aux c'
       else
         match t1, t2 with
         | Types.Var x, _ =>
             if Id.FSet.mem x (Types.FV t2) then None
-            else option_map (cons (x, t2)) (unify (subst x t2 c'))
+            else option_map (cons (x, t2)) (unify_aux (subst (Types.subst_single x t2) c'))
         | _, Types.Var x =>
             if Id.FSet.mem x (Types.FV t1) then None
-            else option_map (cons (x, t1)) (unify (subst x t1 c'))
+            else option_map (cons (x, t1)) (unify_aux (subst (Types.subst_single x t1) c'))
         | Types.Fun t11 t12, Types.Fun t21 t22 =>
-            unify ((t11, t21) :: (t12, t22) :: c')
+            unify_aux ((t11, t21) :: (t12, t22) :: c')
         | _, _ => None
         end
   end.
 Proof.
-  - intros. apply lt_cons.
+  - intros. eauto.
   - intros. apply lt_subst; eauto.
-    intros H.
-    apply Id.FSet.mem_spec in H.
-    congruence.
-  - intros. apply lt_fun.
+    apply Id.FSetProperties.Dec.F.not_mem_iff.
+    eauto.
+  - intros. eauto.
   - intros. apply lt_subst; eauto.
-    intros H.
-    apply Id.FSet.mem_spec in H.
-    congruence.
+    apply Id.FSetProperties.Dec.F.not_mem_iff.
+    eauto.
   - intros. apply lt_subst; eauto.
-    intros H.
-    apply Id.FSet.mem_spec in H.
-    congruence.
+    apply Id.FSetProperties.Dec.F.not_mem_iff.
+    eauto.
   - apply lt_wf.
 Qed.
+
+Definition unify c :=
+  option_map (fold_right
+    (fun p s x => Types.subst s (Types.subst_single (fst p) (snd p) x))
+    Types.Var) (unify_aux c).
 
 Theorem unify_sound : forall c s,
   unify c = Some s -> unifies s c.
 Proof.
   intros c.
+  unfold unify.
   induction c as [[| [t1 t2]] IHc] using (well_founded_induction lt_wf);
-    rewrite unify_equation;
+    rewrite unify_aux_equation;
     intros ? Hunify.
   - inversion Hunify.
     eauto.
@@ -206,51 +175,74 @@ Proof.
         repeat match goal with
         | H : context [if Id.FSet.mem ?x ?s then _ else _] |- _ =>
             let b := fresh in
-            remember (Id.FSet.mem x s) as b;
+            let Heqb := fresh in
+            remember (Id.FSet.mem x s) as b eqn:Heqb;
+            symmetry in Heqb;
             destruct b;
-            [| let H' := fresh in
-               assert (H' : ~Id.FSet.In x s)
-                 by (intros H'; apply Id.FSet.mem_spec in H'; congruence) ]
-        | H : option_map (cons _) (unify ?c) = _ |- _ =>
+            [| apply Id.FSetProperties.Dec.F.not_mem_iff in Heqb ]
+        | H : context [option_map _ (unify_aux ?c)] |- _ =>
             let o := fresh in
             let Heqo := fresh in
-            remember (unify c) as o eqn:Heqo;
-            symmetry in Heqo;
-            destruct o
-        | H : unify ?c = Some ?s |- _ =>
-            assert (unifies s c) by (apply IHc; eauto); clear H
+            remember (unify_aux c) as o eqn:Heqo;
+            destruct o; [ simpl in H; inversion H; subst |]
+        | H : Some ?s = unify_aux ?c |- _ =>
+            assert (unifies (fold_right
+              (fun p s x => Types.subst s (Types.subst_single (fst p) (snd p) x))
+              Types.Var s) c) by
+              (apply IHc; [| rewrite <- H ]; eauto);
+            clear H
+        | H : Forall _ (_ :: _) |- _ => inversion H; clear H; subst
+        | |- Forall _ (_ :: _) => constructor
+        | H : Forall _ (map _ _) |- _ => apply Forall_map in H
+        | H : Forall _ ?l |- Forall _ ?l =>
+            eapply Forall_impl; [| apply H ];
+            intros
         end;
-        repeat (match goal with
-        | _ => rewrite Types.subst_list_Fun in *
-        | _ => rewrite Types.subst_notin_fv in * by eauto
-        | H : Some _ = Some _ |- _ => inversion H; clear H
-        | |- context [Id.eq_dec ?x ?y] => destruct (Id.eq_dec x y)
+        repeat (simpl in *; match goal with
         | H : ~Id.FSet.In ?x (Id.FSet.union ?s1 ?s2) |- _ =>
             assert (~Id.FSet.In x s1) by eauto;
             assert (~Id.FSet.In x s2) by eauto;
             clear H
-        | |- Forall _ (_ :: _) => constructor
-        | H : Forall _ (_ :: _) |- _ => inversion H; clear H
-        | H : Forall _ (map _ _) |- _ => apply Forall_map in H
-        end; simpl in *; subst);
-        solve [ eauto | congruence ].
+        | _ => rewrite Types.subst_subst in *
+        | |- context [Types.subst_single] => unfold Types.subst_single
+        | H : context [Types.subst_single] |- _ => unfold Types.subst_single in *
+        | |- context [Id.eq_dec ?x ?y] => destruct (Id.eq_dec x y)
+        end); simpl in *; try congruence.
+      * f_equal; apply Types.subst_ext; intros;
+          destruct (Id.eq_dec t0 x); simpl; congruence.
+      * f_equal; apply Types.subst_ext; intros;
+          destruct (Id.eq_dec t0 x); simpl; congruence.
 Qed.
 
 Notation moregen s s' :=
-  (exists s0, forall e, Types.subst_list s e = Types.subst_list s0 (Types.subst_list s' e)).
+  (exists s0, forall e, Types.subst s e = Types.subst s0 (Types.subst s' e)).
 
-Lemma moregen_extend : forall subs x t subs',
-  Types.unifies subs (Types.Var x) t ->
-  moregen subs subs' ->
-  moregen subs ((x, t) :: subs').
+Lemma subst_single_preserves_unifies : forall x t0 s c,
+  s x = Types.subst s t0 ->
+  unifies s c ->
+  unifies s (subst (Types.subst_single x t0) c).
 Proof.
-  intros ? x t ? ? Hmoregen.
-  destruct Hmoregen as [ s0 Hmoregen' ].
-  exists s0.
-  intros ?.
-  simpl.
-  rewrite <- Hmoregen'.
-  erewrite Types.subst_preserves_unifies; eauto.
+  intros ? ? ? ? ? H.
+  apply Forall_map.
+  eapply Forall_impl; [| apply H ].
+  intros.
+  simpl in *.
+  repeat rewrite Types.subst_single_preserves_unifies; eauto.
+Qed.
+Hint Resolve subst_single_preserves_unifies.
+
+Lemma moregen_extend : forall s x t s',
+  s x = Types.subst s t ->
+  moregen s s' ->
+  moregen s (fun y => Types.subst s' (Types.subst_single x t y)).
+Proof.
+  intros ? ? ? ? ? H.
+  destruct H as [s'' H].
+  exists s''.
+  intros.
+  rewrite <- Types.subst_subst.
+  rewrite <- H.
+  rewrite Types.subst_single_preserves_unifies; eauto.
 Qed.
 
 Theorem unify_complete : forall c s,
@@ -258,11 +250,15 @@ Theorem unify_complete : forall c s,
   exists s', unify c = Some s' /\ moregen s s'.
 Proof.
   intros c.
+  unfold unify.
   induction c as [[| [t1 t2]] IHc] using (well_founded_induction lt_wf);
-    rewrite unify_equation;
+    rewrite unify_aux_equation;
     intros s Hunifies.
-  - exists nil.
-    simpl.
+  - exists Types.Var.
+    split; eauto.
+    eexists s.
+    intros.
+    rewrite Types.subst_id.  
     eauto.
   - destruct (Types.eq_dec t1 t2).
     + subst.
@@ -281,25 +277,27 @@ Proof.
             [ apply Id.FSet.mem_spec in Heqb;
               exfalso;
               eapply Types.unifies_occur; eauto
-            | let H' := fresh in
-              assert (H' : ~Id.FSet.In x s)
-                by (intros H'; apply Id.FSet.mem_spec in H'; congruence) ]
-        | |- context [unify ?c] =>
-            let H := fresh in
-            assert (H : exists s', unify c = Some s' /\ moregen s s');
+            | apply Id.FSetProperties.Dec.F.not_mem_iff in Heqb ]
+        | |- context [unify_aux ?c] =>
+            assert (H : exists s', option_map (fold_right
+              (fun p s x => Types.subst s (Types.subst_single (fst p) (snd p) x)) Types.Var)
+              (unify_aux c) = Some s' /\ moregen s s');
             [ apply IHc; eauto
             | destruct H as [? [H]];
-              rewrite H ]
-        end;
-        repeat (simpl in *; match goal with
-        | H : Types.Fun _ _ = Types.Fun _ _ |- _ => inversion H; clear H
-        | _ => apply moregen_extend
-        | _ => apply subst_preserves_unifies
-        | _ => rewrite Types.subst_list_Bool in *
-        | _ => rewrite Types.subst_list_Fun in *
+              let o := fresh in
+              let Heqo := fresh in
+              remember (unify_aux c) as o eqn:Heqo;
+              destruct o;
+              [ simpl in Heqo; inversion Heqo; subst
+              | simpl in H; congruence ]]
+        end; simpl in *;
+        repeat (match goal with
+        | |- Forall _ (_ :: _) => constructor
         | |- exists _, Some _ = Some _ /\ _ =>
             eexists;
             split; [ reflexivity |]
-        end);
-        solve [ eauto | congruence ].
+        | H : Some _ = Some _ |- _ => inversion H; clear H
+        | |- _ => apply moregen_extend
+        end; simpl in *; subst);
+        try solve [ eauto | congruence ].
 Qed.
